無駄な記述が多そう

practice/coq/deBruijn/ocaml/src/eval.mli
@@ -9,8 +9,6 @@ type 'a option =
 
 
 
-val add : nat -> nat -> nat
-
 module Nat :
  sig
   val pred : nat -> nat
@@ -29,7 +27,7 @@ type deBruijn =
 | App of deBruijn * deBruijn
 | Abs of char list * deBruijn
 
-val shift : nat -> nat -> deBruijn -> deBruijn
+val shift : nat -> deBruijn -> deBruijn
 
 val subst : nat -> deBruijn -> deBruijn -> deBruijn
 
